erasure/theories/SafeErasureFunction.v
@@ -182,7 +182,7 @@ Next Obligation.
 
      eapply conv_context_refl; eauto. econstructor.
 
-     eapply PCUICConversion.conv_sym, red_conv; eauto.
+     eapply conv_sym, red_conv; eauto.
   ++ sq. etransitivity. eassumption.
 
      eapply context_conversion_red; eauto. econstructor.
@@ -191,7 +191,7 @@ Next Obligation.
 
      econstructor.
 
-     eapply PCUICConversion.conv_sym, red_conv; eauto.
+     eapply conv_sym, red_conv; eauto.
 Qed.
 
 Next Obligation.
@@ -288,7 +288,7 @@ Next Obligation.
 
     eapply leq_universe_prop in l0 as []; cbn; eauto.
     eapply leq_universe_prop in l as []; cbn; eauto.
-    eauto using typing_wf_local.
+    reflexivity. eauto using typing_wf_local.
 Qed.
 
 (* Program Definition is_erasable (Sigma : PCUICAst.global_env_ext) (HΣ : ∥wf_ext Sigma∥) (Gamma : context) (HΓ : ∥wf_local Sigma Gamma∥) (t : PCUICAst.term) : *)
