pcuic/theories/PCUICLiftSubst.v
@@ -1649,3 +1649,10 @@ Proof.
     + simpl. repeat f_equal; try lia.
     + simpl. apply IHΓ'; simpl in *; (lia || congruence).
 Qed.
+
+Fixpoint subst_app (t : term) (us : list term) : term :=
+  match t, us with
+  | tLambda _ A t, u :: us => subst_app (t {0 := u}) us
+  | _, [] => t
+  | _, _ => mkApps t us
+  end.
