pcuic/theories/TemplateToPCUICCorrectness.v
@@ -1344,7 +1344,7 @@ Proof.
     eapply typing_wf in X; eauto. destruct X.
     clear H1 X0 H H0. revert H2.
     induction X1. econstructor; eauto.
-    (* Need updated typing_spine in template-coq *) admit.
+    (* Need updated typing_spine in template-coq *) admit. reflexivity.
     simpl in p.
     destruct (TypingWf.typing_wf _ wfΣ _ _ _ typrod) as [wfAB _].
     intros wfT.
